src/association_list.v
@@ -1,0 +1,77 @@
+Require Import Mmx.ast.
+Require Import Mmx.binary.
+Require Import List.
+Import ListNotations.
+Require Import Bool.
+Require Import Nat Arith.
+
+Definition tag_opcode_assoc :=
+  list (tag * structure_op  * nat).
+
+Definition M A := option A.
+
+Definition ret {A} (a : A) : M A := Some a.
+
+Definition bind {A B} (ma : M A)(k : A -> M B): M B :=
+  match ma with
+  | Some a => k a
+  | None => None
+  end.
+
+Notation "'let!' x ':=' ma 'in' k" := (bind ma (fun x => k)) (at level 30).   
+
+
+Fixpoint lookup (t : tag) (l : tag_opcode_assoc) : option nat :=
+  match l with
+    | [] => None
+    | (t',s,n) :: tl => if tag_beq t t' 
+                        then Some n
+                        else lookup t tl
+  end.
+Fixpoint lookdown (n : nat) (l : tag_opcode_assoc) : option (tag * structure_op) :=
+  match l with
+    | [] => None
+    | (t,s,n') :: tl => if  beq_nat n n'
+                        then Some (t,s)
+                        else lookdown n tl
+  end.
+
+
+
+Definition encdec : tag_opcode_assoc := 
+  [
+    (Arith ADD Signed, [Reg_s 8;Reg_s 8;Reg_s 8],10);
+      (Arith SUB Signed, [Reg_s 8;Reg_s 8;Reg_s 8],11)
+  ].    
+
+
+Print reflect.
+Lemma test_reflect : True -> reflect True true.
+Proof.
+  exact (ReflectT True).
+Qed.
+
+
+Definition tag_to_nat (t : tag) : option nat := lookup t encdec.
+
+Definition nat_to_tag (n : nat) : option (tag*structure_op) := lookdown n encdec.
+
+Theorem lookdown_lookup : forall (n : nat) (s : structure_op) (t : tag),
+    lookdown n encdec = Some (t,s) -> lookup t encdec = Some n.
+Proof.
+Admitted.
+
+Theorem lookup_lookdown : forall (n : nat) (t : tag) (s : structure_op),
+    lookup t encdec = Some n -> lookdown n encdec = Some (t,s).
+  Admitted.
+
+
+
+  
+
+  
+
+
+
+
+
