src/encodeDecode.v
@@ -1,0 +1,64 @@
+Require Import Mmx.ast.
+Require Import Mmx.binary.
+Require Import Mmx.association_list.
+Require Import List.
+Import ListNotations.
+
+
+(* ------------------------------- Encode --------------------------- *)
+
+Fixpoint encode_operandes_rec (o : operands) (res : list bool) : option (list bool) :=
+  match o with
+  | [] => Some res
+  | (op,size) :: next => let! op_n := (match op with
+                                      | imm n => n_bit size n 
+                                      | reg n => n_bit size n
+                                      end) in
+                          encode_operandes_rec next (res ++ op_n)
+  end.
+Definition encode_operandes (o : operands) : option (list bool) :=
+  encode_operandes_rec o [].
+
+
+Definition encode (i : instr) : option binary_instruction :=
+  match i with
+  | mk_instr t op => let! nat_tag := tag_to_nat t in
+                     let! binary_tag := n_bit 8 nat_tag in 
+                     let! binary_op := encode_operandes op in
+                     Some (binary_tag ++ binary_op)
+  end.
+
+
+
+
+
+(* ----------------------------- Decode ------------------------- *)
+Fixpoint get_first_n_bit  (bi : list bool) (size : nat) : (list bool*list bool) :=
+  match size with
+  | 0 => ([],bi)
+  | S n => match bi with
+           | h :: tl => match get_first_n_bit tl n with
+                        | (l1,l2) => (h :: l1,l2)
+                        end
+           | [] => ([],[])
+           end
+  end.
+
+
+Fixpoint decode_operandes (op_binary : list bool) (s : structure_op) : operands :=
+  match s with
+  | [] => []
+  | elem_struct :: next => let res := match elem_struct with
+                                              | Imm_s siz => let (a,b) := get_first_n_bit op_binary siz in
+                                                             (a,siz,b,imm) 
+                                              | Reg_s siz => let (a,b) := get_first_n_bit op_binary siz in
+                                                             (a,siz,b,reg) 
+                                      end in
+                           match res with
+                           | (l,siz,reste,construct) => let op := bit_n l in
+                                                        (construct op, siz) :: decode_operandes reste next
+                           end
+  end.
+
+
+
